Iterator/Combinators/Drop.lean
@@ -4,25 +4,18 @@ Released under Apache 2.0 license as described in the file LICENSE.
 Authors: Paul Reichert
 -/
 prelude
-import Iterator.SimpleIterator
+import Iterator.Basic
+import Iterator.Consumers.Collect
 
 /-!
 This file provides the iterator combinator `Iter.drop`.
 -/
 
-variable {α : Type u} {m : Type w → Type w'} {β : Type v}
+variable {α : Type w} {m : Type w → Type w'} {β : Type v}
 
 structure Drop (α : Type u) where
   remaining : Nat
   inner : α
-
-instance [Monad m] [Iterator α m β] : SimpleIterator (Drop α) m β where
-  step it := matchStep (m := m) it.inner
-      (fun it' b => match it.remaining with
-        | 0 => pure <| .yield ⟨0, it'⟩ b
-        | remaining' + 1 => pure <| .skip ⟨remaining', it'⟩)
-      (fun it' => pure <| .skip ⟨it.remaining, it'⟩)
-      (pure <| .done)
 
 /--
 Given an iterator `it` and a natural number `n`, `it.drop n` is an iterator that forwards all of
@@ -50,26 +43,66 @@ _TODO_: prove `Productive`
 Currently, this combinator incurs an additional O(1) cost with each output of `it`, even when the iterator
 does not drop any elements anymore.
 -/
-def Iter.drop [Iterator α m β] [Monad m] [ComputableUnivLE.{u, w}] {small : ComputableSmall.{w} α}
-    (n : Nat) (it : Iter (α := α) m β (small := small)) :=
-  toIter (α := Drop α) m <| Drop.mk n it.inner
+def Iter.drop [Iterator α m β]
+    (n : Nat) (it : Iter (α := α) m β) :=
+  toIter (Drop.mk n it.inner) m β
 
-def Drop.rel (m : Type w → Type w') [Iterator α m β] : Drop α → Drop α → Prop :=
-  InvImage FiniteIteratorWF.lt (finiteIteratorWF (m := m) ∘ Drop.inner)
+def Drop.innerIter {α : Type w} {m : Type w → Type w'} {β : Type v}
+    (it : Iter (α := Drop α) m β) : Iter (α := α) m β :=
+  toIter it.inner.inner m β
 
-instance [Iterator α m β] [Monad m] [Finite α m] : SimpleIterator.Finite (Drop α) m where
+inductive Drop.PlausibleStep [Iterator α m β] (it : Iter (α := Drop α) m β) :
+    (step : IterStep (Iter (α := Drop α) m β) β) → Prop where
+  | drop : ∀ {it' out k}, (innerIter it).plausible_step (.yield it' out) →
+      it.inner.remaining = k + 1 → PlausibleStep it (.skip (it'.drop k))
+  | skip : ∀ {it'}, (innerIter it).plausible_step (.skip it') →
+      PlausibleStep it (.skip (it'.drop it.inner.remaining))
+  | done : (innerIter it).plausible_step .done → PlausibleStep it .done
+  | yield : ∀ {it' out}, (innerIter it).plausible_step (.yield it' out) →
+      it.inner.remaining = 0 → PlausibleStep it (.yield (it'.drop 0) out)
+
+instance [Iterator α m β] {it : Iter (α := Drop α) m β} :
+    Small.{w} (Subtype <| Drop.PlausibleStep it) := sorry
+
+instance Drop.instIterator [Monad m] [Iterator α m β] : Iterator (Drop α) m β where
+  plausible_step := Drop.PlausibleStep
+  step_small := inferInstance
+  step it := do
+    match (← (innerIter it).stepH).inflate (small := _) with
+    | .yield it' out h =>
+      match h' : it.inner.remaining with
+      | 0 => pure <| .deflate <| .yield (it'.drop 0) out (.yield h h')
+      | k + 1 => pure <| .deflate <| .skip (it'.drop k) (.drop h h')
+    | .skip it' h =>
+      pure <| .deflate <| .skip (it'.drop it.inner.remaining) (.skip h)
+    | .done h =>
+      pure <| .deflate <| .done (.done h)
+
+def Drop.rel (m : Type w → Type w') [Iterator α m β] [Finite α m] :
+    Iter (α := Drop α) m β → Iter (α := Drop α) m β → Prop :=
+  InvImage Iter.TerminationMeasures.Finite.rel (Iter.finitelyManySteps ∘ Drop.innerIter)
+
+instance Take.instFinitenessRelation [Iterator α m β] [Monad m] [Finite α m] :
+    FinitenessRelation (Drop α) m where
   rel := Drop.rel m
   wf := by
     apply InvImage.wf
+    apply InvImage.wf
     exact Finite.wf
   subrelation {it it'} h := by
-    simp only [SimpleIterator.step] at h
-    obtain ⟨_, _, hy, h⟩ | ⟨_, hs, h⟩ | ⟨hd, h⟩ := successor_matchStep h
-    · split at h
-      · cases successor_yield.mp h
-        exact Or.inl ⟨_, hy⟩
-      · cases successor_skip.mp h
-        exact Or.inl ⟨_, hy⟩
-    · cases successor_skip.mp h
-      exact Or.inr hs
-    · cases successor_done.mp h
+    obtain ⟨step, h, h'⟩ := h
+    cases h'
+    case drop it' h' _ =>
+      cases h
+      apply Iter.plausible_successor_of_yield
+      exact h'
+    case skip it' h' =>
+      cases h
+      apply Iter.plausible_successor_of_skip
+      exact h'
+    case done h' =>
+      cases h
+    case yield it' out h' h'' =>
+      cases h
+      apply Iter.plausible_successor_of_yield
+      exact h'
