Iterator/Lemmas/Producer.lean
@@ -4,38 +4,41 @@ import Iterator.Lemmas.Consumer
 
 section ListIterator
 
-variable {m : Type v → Type v} [Monad m] [LawfulMonad m] {β : Type v}
+variable {m : Type w → Type w'} [Monad m] [LawfulMonad m] {β : Type w}
 
 theorem List.step_iter_nil :
-    (([] : List β).iter m).step = pure ⟨.done, by simp [Iterator.plausible_step, List.iter, Iter.plausible_step, IterStep.map]⟩ := by
-  simp only [iter, Iter.step, Iter.stepH, Iter.Step.ofInternal, IterStep.map, id_eq, Iterator.step,
-    map_pure, USquash.inflate_deflate]
+    (([] : List β).iter m).step =
+      pure ⟨.done, by simp [Iterator.plausible_step, List.iter, Iter.plausible_step, IterStep.map]⟩ := by
+  simp only [iter, Iter.step, Iter.stepH, IterStep.map, id_eq, Iterator.step, map_pure, USquash.inflate_deflate]
   congr
-  unfold Iter.stepH.proof_1 -- :(
-  rw [inner_toIter]
-  simp
+  simp [toIter]
 
 theorem List.step_iter_cons {x : β} {xs : List β} :
     ((x :: xs).iter m).step = pure ⟨.yield (xs.iter m) x, by simp [List.iter, Iter.plausible_step, Iterator.plausible_step, IterStep.map]⟩ := by
-  simp only [iter, Iter.step, Iter.stepH, Iter.Step.ofInternal, IterStep.map, id_eq, Iterator.step,
+  simp only [iter, Iter.step, Iter.stepH, IterStep.map, id_eq, Iterator.step,
     map_pure, USquash.inflate_deflate]
   congr
-  unfold Iter.stepH.proof_1
-  rw [inner_toIter]
-  simp
+  simp [toIter]
 
-private theorem List.toArray_iter.aux {l : List β} {acc : Array β} :
-    Iter.toArray.go (l.iter m) acc = pure (acc ++ l.toArray) := by
-  induction l generalizing acc with
+theorem ListIterator.toArrayMapped_eq {β : Type w} {γ : Type w} {f : β → m γ}
+    {l : List β} :
+    IteratorToArray.toArrayMapped f (l.iter m) = List.toArray <$> l.mapM f := by
+  rw [LawfulIteratorToArray.lawful]
+  induction l with
   | nil =>
-    rw [Iter.toArray.go]
+    rw [Iter.DefaultConsumers.toArrayMapped_of_step]
     simp [List.step_iter_nil]
   | cons x xs ih =>
-    rw [Iter.toArray.go]
-    simp [List.step_iter_cons, ih]
+    rw [Iter.DefaultConsumers.toArrayMapped_of_step]
+    simp [List.step_iter_cons, List.mapM_cons, pure_bind, ih]
 
 theorem List.toArray_iter {l : List β} :
     Iter.toArray (l.iter m) = pure l.toArray := by
-  simp [Iter.toArray, List.toArray_iter.aux]
+  simp only [Iter.toArray, ListIterator.toArrayMapped_eq]
+  rw [mapM_pure, map_pure, List.map_id']
+
+theorem List.toList_iter {l : List β} :
+    Iter.toList (l.iter m) = pure l := by
+  rw [← Iter.toList_toArray, List.toArray_iter, map_pure, toList_toArray]
 
 end ListIterator
